The MCH is merely a proxy in front of a PIO Memory

specs/x86/MCH/MemStorage.v
@@ -1,5 +1,7 @@
+Require Import Coq.Arith.Arith.
 Require Import FreeSpec.Specs.Memory.
 Require Import FreeSpec.Interface.
+Require Import FreeSpec.Interp.
 Require Import FreeSpec.Control.
 Require Import FreeSpec.Control.Function.
 Require Import FreeSpec.MonadInterp.
@@ -7,62 +9,179 @@ Require Import FreeSpec.Control.State.
 Require Import FreeSpec.Control.Classes.
 Require Import FreeSpec.Control.Identity.
 Require Import FreeSpec.WEq.
+Require Import Omega.
 
 Local Open Scope free_weq_scope.
 Local Open Scope free_control_scope.
 
-Inductive MemStorage_int
+Inductive MSi
           (n:  nat)
   : Interface :=
-| read_ms (addr:  mem n)
-  : MemStorage_int n byte
-| write_ms (addr:  mem n)
-           (val:   byte)
-  : MemStorage_int n unit.
+| read_byte (addr:  mem n)
+  : MSi n byte
+| read_word (addr:  mem n)
+  : MSi n word
+| read_lword (addr:  mem n)
+  : MSi n lword
+| write_byte (addr:  mem n)
+             (val:   byte)
+  : MSi n unit
+| write_word (addr:  mem n)
+             (val:   word)
+  : MSi n unit
+| write_lword (addr:  mem n)
+              (val:   lword)
+  : MSi n unit.
 
-Arguments read_ms {n} (addr).
-Arguments write_ms {n} (addr val).
+Arguments read_byte  {n} (addr).
+Arguments read_word  {n} (addr).
+Arguments read_lword {n} (addr).
+Arguments write_byte  {n} (addr val).
+Arguments write_word  {n} (addr val).
+Arguments write_lword {n} (addr val).
 
-Definition MemStorage_state
+Definition MSs
            (n:  nat)
   := mem n
      -> byte.
 
-Definition MemStorage_state_weq
+Definition MSs_weq
            {n:             nat}
-           (store store':  MemStorage_state n)
+           (store store':  MSs n)
   : Prop :=
   forall (addr: mem n),
     store addr == store' addr.
 
-Instance MemStorage_state_WEq
+Instance MSs_WEq
          (n:  nat)
-  : WEq (MemStorage_state n) :=
-  { weq := @MemStorage_state_weq n
+  : WEq (MSs n) :=
+  { weq := @MSs_weq n
   }.
 
-Definition MemStorage_init
+Definition MSs_init
            (n:  nat)
-  : MemStorage_state n :=
-  pure (zero 8).
+  : MSs n :=
+  pure (0: byte).
 
-Definition MemStorage_interp
+Definition nxt
+           {n:  nat}
+           (x:  mem n)
+  : mem n :=
+  add x (box n 1).
+
+Lemma nxt_neq
+      {n:  nat}
+      (x:  mem n)
+      (H:  1 < n)
+  : ~ weq x (nxt x).
+Proof.
+  unfold nxt.
+  unfold add.
+  unfold box, unbox.
+  intros [Heq].
+  destruct x as [x Hx].
+  unfold mem_val in Heq.
+  rewrite Nat.mod_1_l in Heq.
+  + destruct (Nat.eq_dec (x + 1) (2 ^ n)).
+    ++ rewrite e in Heq.
+       rewrite Nat.mod_same in Heq.
+       subst.
+       rewrite Nat.add_0_l in e.
+       assert (Hn:  n = 0). {
+         rewrite <- (Nat.pow_0_r 2) in e at 1.
+         apply Nat.pow_inj_r in e.
+         symmetry; exact e.
+         omega.
+       }
+       subst.
+       inversion H.
+       apply Nat.neq_sym.
+       apply lt_0_neq.
+       apply pow_pos.
+       omega.
+    ++ assert (Hn:  x + 1 < 2 ^ n) by omega.
+       rewrite Nat.mod_small in Heq; [| exact Hn ].
+       omega.
+  + apply Nat.pow_gt_1; omega.
+Qed.
+
+Definition MS_interp
            {n:  nat}
            {A:  Type}
-           (i:  MemStorage_int n A)
-  : State (MemStorage_state n) A :=
+           (i:  MSi n A)
+  : State (MSs n) A :=
   match i with
-  | read_ms addr
-    => gets (fun store => store addr)
-  | write_ms addr val
-    => modify (fun store addr'
-               => if addr ?= addr'
-                  then val
-                  else store addr')
+  | read_byte addr
+    => gets (fun store
+             => store addr)
+  | read_word addr
+    => gets (fun store
+             => join_bytes_to_word (store (nxt addr))
+                                   (store addr))
+  | read_lword addr
+    => gets (fun store
+             => join_bytes_to_lword (store (nxt (nxt (nxt addr))))
+                                    (store (nxt (nxt addr)))
+                                    (store (nxt addr))
+                                    (store addr))
+  | write_byte addr val
+    => modify (fun store
+               => fun addr'
+                  => if addr' ?= addr
+                     then val
+                     else store addr')
+  | write_word addr val
+    => modify (fun store
+               => fun addr'
+                  => if addr' ?= addr
+                     then lower_word_half val
+                     else if addr' ?= nxt addr
+                          then upper_word_half val
+                          else store addr')
+  | write_lword addr val
+    => modify (fun store
+               => fun addr'
+                  => if addr' ?= addr
+                     then lword_quarter_1 val
+                     else if addr' ?= nxt addr
+                          then lword_quarter_2 val
+                          else if addr' ?= nxt (nxt addr)
+                               then lword_quarter_3 val
+                               else if addr' ?= nxt (nxt (nxt addr))
+                                    then lword_quarter_4 val
+                                    else store addr')
   end.
 
 Instance memstorage_MonadInterp
          (n:  nat)
-  : MonadInterp (MemStorage_int n) (State (MemStorage_state n)) :=
-  { interpret := @MemStorage_interp n
+  : MonadInterp (MSi n) (State (MSs n)) :=
+  { interpret := @MS_interp n
   }.
+
+Definition MSInterp
+           {n:  nat}
+           (x:  MSs n)
+  : Interp (MSi n) :=
+  monad_state_interp (MSs_init n).
+
+Require Import FreeSpec.Program.
+Local Open Scope free_prog_scope.
+
+Fact write_then_read
+     {n:  nat}
+     (H:  1 < n)
+     (x:  MSs n)
+     (a:  mem n)
+     (v:  word)
+  : evalProgram (MSInterp x) ([write_word a v] ;; [read_word a]) == v.
+Proof.
+  Opaque weq_bool.
+  cbn.
+  repeat rewrite weq_bool_refl.
+  rewrite (weq_bool_false_rewrite (nxt a) a).
+  rewrite <- join_bytes_upper_lower_eq.
+  reflexivity.
+  apply not_weq_sym.
+  apply (nxt_neq a).
+  exact H.
+Qed.
