specs/x86/MCH/MCH.v
@@ -4,6 +4,7 @@ Require Import FreeSpec.Specs.Address.
 Require Import FreeSpec.Interface.
 Require Import FreeSpec.Undefined.
 Require Import FreeSpec.Refine.
+Require Import FreeSpec.Compose.
 Require Import FreeSpec.Control.
 Require Import FreeSpec.Control.Classes.
 Require Import FreeSpec.Control.State.
@@ -12,9 +13,11 @@ Require Import FreeSpec.WEq.
 Require Import FreeSpec.Compose.
 Require Import FreeSpec.Specs.Bitfield.
 Require Import FreeSpec.Specs.x86.MCH.SMRAMC.
+Require Import FreeSpec.Specs.x86.MCH.MemStorage.
 Require Import FreeSpec.PropBool.
 
 Local Open Scope free_scope.
+Local Open Scope free_prog_scope.
 Local Open Scope free_control_scope.
 
 (** * Interface
@@ -23,111 +26,23 @@ Local Open Scope free_control_scope.
 
 Inductive MCHi
   : Interface :=
-| PIO_in32 (port: word)
+| PIO_in32 (port:  word)
   : MCHi lword
-| PIO_out32 (port: word)
-            (val:  lword)
+| PIO_in16 (port:  word)
+  : MCHi word
+| PIO_in8 (port:  word)
+  : MCHi byte
+| PIO_out32 (port:  word)
+            (val:   lword)
   : MCHi unit
-| IO_read (addr: address_64B_aligned)
-  : MCHi (mem (64 Bytes))
-| IO_write (addr: address_64B_aligned)
-           (val:  mem (64 Bytes))
+| PIO_out16 (port:  word)
+            (val:   word)
+  : MCHi unit
+| PIO_out8 (port:  word)
+            (val:  byte)
   : MCHi unit.
 
-(** * Hardware Specification
-
- *)
-
-Inductive ConfAddr
-  : Type :=
-| confaddr (bus:        nat)
-           (device:     nat)
-           (function:   nat)
-           (register:   nat)
-           (pci_enable: bool)
-  : ConfAddr.
-
-Definition confaddr_eqb
-           (c c': ConfAddr)
-  : bool :=
-  match c, c' with
-  | confaddr b d f r p, confaddr b' d' f' r' p'
-    =>  Nat.eqb b b'
-     && Nat.eqb d d'
-     && Nat.eqb f f'
-     && Nat.eqb r r'
-     && Bool.eqb p p'
-  end.
-
-Fact confaddr_eqb_refl
-     (c: ConfAddr)
-  : confaddr_eqb c c = true.
-Proof.
-  destruct c.
-  unfold confaddr_eqb.
-  repeat rewrite <- EqNat.beq_nat_refl.
-  rewrite Bool.eqb_reflx.
-  reflexivity.
-Qed.
-
-Instance confaddr_PropBoolP
-  : PropBool2 (@eq ConfAddr) (confaddr_eqb) :=
-  {
-  }.
-  intros c c'; split.
-  + intros H.
-    destruct c; destruct c'.
-    unfold confaddr_eqb in H.
-    apply Bool.andb_true_iff in H; destruct H as [H H'].
-    apply Bool.andb_true_iff in H; destruct H as [H H''].
-    apply Bool.andb_true_iff in H; destruct H as [H H'''].
-    apply Bool.andb_true_iff in H; destruct H as [H H''''].
-    apply EqNat.beq_nat_true in H.
-    apply EqNat.beq_nat_true in H''.
-    apply EqNat.beq_nat_true in H'''.
-    apply EqNat.beq_nat_true in H''''.
-    apply Bool.eqb_prop in H'.
-    subst.
-    reflexivity.
-  + intros Heq.
-    rewrite Heq.
-    rewrite confaddr_eqb_refl.
-    reflexivity.
-Defined.
-
-Definition SMRAMC_Addr
-  : ConfAddr :=
-  confaddr 0 16 0 22 true. (* 16h *)
-
-Definition ConfAddr_bf
-  : Bitfield 32 ConfAddr :=
-  skip 1                 :;
-  register :<- field 7    ;
-  function :<- field 3    ;
-  device   :<- field 5    ;
-  bus      :<- field 8    ;
-  skip 7                 :;
-  pci      :<- bit        ;
-  bf_pure (confaddr bus device function register pci).
-
-Definition parse_confaddr
-           (w: lword)
-  : ConfAddr :=
-  parse ConfAddr_bf w.
-
-Inductive io_write32_target
-  : Type :=
-| ConfAddr_target
-| ConfData_target
-| Invalid_target.
-
-Axiom word_to_target
-  : word -> option io_write32_target.
-
-Record MCHs :=
-  { confAddr: ConfAddr
-  ; smramc: SMRAMC
-  }.
+Definition MCHs := unit.
 
 Instance mchs_WEq
   : WEq MCHs :=
@@ -138,7 +53,7 @@ Instance mchs_WEq
     cannot find the typeclass instance any longer.
 
  *)
-Notation "'MCHm' A":= (StateT MCHs (Program (MCHi <+> Undefined)) A)
+Notation "'MCHm' A":= (StateT MCHs (Program (MSi 16 <+> Undefined)) A)
                         (at level 30).
 
 (* We have to help a little Coq here. See #16 for more information on
@@ -148,57 +63,54 @@ Definition mch_undefined
   : MCHm A :=
   undef (UndefMonad:=undefmonad_Trans _ _).
 
-Definition update_confaddr
-           (ca: ConfAddr)
+Definition pio_out8
+           (x:  word)
+           (v:  byte)
   : MCHm unit :=
-  modify (fun s
-          => {| confAddr := ca
-              ; smramc := smramc s
-              |}).
+   '[ileft (write_byte x v)].
 
-Definition get_confaddr
-  : MCHm ConfAddr :=
-  gets confAddr.
-
-Definition update_smramc
-           (reg: SMRAMC)
+Definition pio_out16
+           (x:  word)
+           (v:  word)
   : MCHm unit :=
-  modify (fun s
-          => {| confAddr := confAddr s
-              ; smramc := reg
-              |}).
-
-Definition get_smramc
-  : MCHm SMRAMC :=
-  gets smramc.
+  '[ileft (write_word x v)].
 
 Definition pio_out32
-           (x: word)
-           (val: lword)
+           (x:  word)
+           (v:  lword)
   : MCHm unit :=
-  match word_to_target x with
-  | Some ConfAddr_target
-    => update_confaddr (parse_confaddr val)
-  | Some ConfData
-    => confaddr <- get_confaddr                                      ;
-       match confaddr with
-       | confaddr 0 16 0 97 (* 61h *) true (* SMRAMC *)
-         => (* update_smramc (parse_smramc val) *)
-             mch_undefined
-       | _
-         => mch_undefined
-       end
-  | Nothing (* An invalid IO out access is just ignore by the MCH   *)
-    => pure tt
-  end.
+  '[ileft (write_lword x v)].
+
+Definition pio_in8
+           (x:  word)
+  : MCHm byte :=
+   '[ileft (read_byte x)].
+
+Definition pio_in16
+           (x:  word)
+  : MCHm word :=
+   '[ileft (read_word x)].
+
+Definition pio_in32
+           (x:  word)
+  : MCHm lword :=
+   '[ileft (read_lword x)].
 
 Definition mch_specs
-  : StatefulRefinement MCHi (MCHi <+> Undefined) MCHs :=
+  : StatefulRefinement MCHi (MSi 16 <+> Undefined) MCHs :=
   fun (A: Type)
       (i: MCHi A)
   => match i with
+     | PIO_out8 x val
+       => pio_out8 x val
+     | PIO_out16 x val
+       => pio_out16 x val
      | PIO_out32 x val
        => pio_out32 x val
-     | _
-       => mch_undefined
+     | PIO_in8 x
+       => pio_in8 x
+     | PIO_in16 x
+       => pio_in16 x
+     | PIO_in32 x
+       => pio_in32 x
      end.
